src/Init/Data/Int/Lemmas.lean
@@ -478,6 +478,8 @@ theorem eq_one_of_mul_eq_self_left {a b : Int} (Hpos : a ≠ 0) (H : b * a = a) 
 theorem eq_one_of_mul_eq_self_right {a b : Int} (Hpos : b ≠ 0) (H : b * a = b) : a = 1 :=
   Int.eq_of_mul_eq_mul_left Hpos <| by rw [Int.mul_one, H]
 
+theorem pow_succ (b : Int) (e : Nat) : b ^ (e+1) = (b ^ e) * b := rfl
+
 /-! NatCast lemmas -/
 
 /-!
